WIP: editing simulation

theories/simulation_local.v
@@ -4,137 +4,148 @@ From iris.algebra Require Import cmra.
 From stbor Require Import simulation.
 
 Section local.
-Context {A: cmraT}.
+Context {A: ucmraT}.
 Variable (wsat: A → state → state → Prop).
 Variable (vrel: A → expr → expr → Prop).
 Variable (fns_src fns_tgt: fn_env).
+Variable (Φinit: A → state → state → Prop).
 
 Section local_step.
-Variable (φ: A → call_id → call_id_stack → state → call_id → call_id_stack → state → Prop).
-Variable (c_src: call_id) (cids_entry_src: call_id_stack)
-         (c_tgt: call_id) (cids_entry_tgt: call_id_stack).
+(* Variable (c_src: call_id) (cids_entry_src: call_id_stack)
+         (c_tgt: call_id) (cids_entry_tgt: call_id_stack). *)
 
 (* TODO: encode what it means for the context to not contain our private tags! *)
 (* TODO: how do we know we're at the top of the stack? *)
-Inductive _sim_local
-  (sim_local : A → A → expr → state → expr → state → Prop)
+Inductive _sim_fn_body
+  (sim_fn_body : A → A → expr → state → expr → state → Prop)
   (r_f r: A) : expr → state → expr → state → Prop :=
 (* If src is stuck, then anything is related *)
-| sim_local_stuck e_src σ_src e_tgt σ_tgt
+| sim_fn_body_stuck e_src σ_src e_tgt σ_tgt
     (STUCK: stuck e_src (mkConfig fns_src σ_src))
-    : _sim_local sim_local r_f r e_src σ_src e_tgt σ_tgt
+    : _sim_fn_body sim_fn_body r_f r e_src σ_src e_tgt σ_tgt
 (* If tgt makes 1 step, src can make some step *)
-| sim_local_step e_src σ_src e_tgt σ_tgt
+| sim_fn_body_step e_src σ_src e_tgt σ_tgt
     (STEP: ∀ e_tgt' cfg_tgt',
-      ✓ (r ⋅ r_f) →
-      (* wsat (r ⋅ r_f) σ_src σ_tgt → *)
-      φ r c_src cids_entry_src σ_src c_tgt cids_entry_tgt σ_tgt →
-      (* if tgt can makes 1 step *)
+      (* if tgt can locally make 1 step *)
       (e_tgt, (mkConfig fns_tgt σ_tgt)) ~t~> (e_tgt', cfg_tgt') →
-      (* then we locally can makes some step and still preserve the frame r_f,
-        and the simulation continues. *)
-      ∃ e_src' cfg_src' r',
+      (* then we locally can makes some step *)
+      ∃ e_src' cfg_src',
         (e_src, (mkConfig fns_src σ_src)) ~t~>* (e_src', cfg_src') ∧
-        ✓ (r' ⋅ r_f) ∧
-        (* wsat (r' ⋅ r_f) cfg_src'.(cst) cfg_tgt'.(cst) ∧ *)
-        φ r' c_src cids_entry_src cfg_src'.(cst) c_tgt cids_entry_tgt cfg_tgt'.(cst) ∧
-        sim_local r_f r' e_src' cfg_src'.(cst) e_tgt' cfg_tgt'.(cst))
-    : _sim_local sim_local r_f r e_src σ_src e_tgt σ_tgt
+        sim_fn_body r_f r e_src' cfg_src'.(cst) e_tgt' cfg_tgt'.(cst))
+    : _sim_fn_body sim_fn_body r_f r e_src σ_src e_tgt σ_tgt
 (* If tgt prepares to make a call to [name], src should be able to make the same
   call. Here we do not want to step into the call of [name], but to step over
-  it. To make the call, we need to re-establish
+  it. To make such a call, we need to re-establish
  `wsat (r ⋅ r_f) cfg_src.(cst) σ_tgt`. Then after the call we can assume that:
   - the context K_src/tgt did not change
   - the call id stack did not change
   - the framed resources r ⋅ r_f did not change
-  - the invariant is re-established by [name] for some new frame and new states. *)
-| sim_local_step_over_call K_src K_tgt name e_src el_src el_tgt σ_src
+  - wsat is re-established by [name] for some new frame and new states. *)
+| sim_fn_body_step_over_call K_src K_tgt name e_src el_src el_tgt σ_src rc rv
     cfg_src σ_tgt
     (STEPS: (e_src, (mkConfig fns_src σ_src)) ~t~>*
             (fill K_src (Call #(LitFnPtr name) el_src), cfg_src))
     (VALS: Forall (λ ei, terminal ei) el_src)
     (VALT: Forall (λ ei, terminal ei) el_tgt)
-    (VALEQ: Forall2 (vrel (r ⋅ r_f)) el_src el_tgt)
-    (VALID: ✓ (r ⋅ r_f))
-    (INV: wsat (r ⋅ r) cfg_src.(cst) σ_tgt)
+    (VALEQ: Forall2 (vrel (rv)) el_src el_tgt)
+    (VALID: ✓ (r_f ⋅ rc ⋅ rv))
+    (INV: wsat (r_f ⋅ rc ⋅ rv) cfg_src.(cst) σ_tgt)
     (RET: ∀ v_src v_tgt r' cfg_src' cfg_tgt',
       (* For any new resource r' that is compatible with our local resource r and frame r_f *)
-      ✓ (r ⋅ r' ⋅ r_f) →
+      ✓ (r_f ⋅ rc ⋅ r') →
       (* and wsat holds for the composed resource + pair of physical states, *)
-      wsat (r ⋅ r' ⋅ r_f) cfg_src'.(cst) cfg_tgt'.(cst) →
+      wsat (r_f ⋅ rc ⋅ r') cfg_src'.(cst) cfg_tgt'.(cst) →
       (* and the returned values are related w.r.t. (r ⋅ r' ⋅ r_f) *)
-      vrel (r ⋅ r' ⋅ r_f) (of_val v_src) (of_val v_tgt) →
-      (* stack unchanged *)
+      vrel (r_f ⋅ rc ⋅ r') (of_val v_src) (of_val v_tgt) →
+      (* (* stack unchanged *)
       cfg_src'.(cst).(scs) = cfg_src.(cst).(scs) →
-      cfg_tgt'.(cst).(scs) = σ_tgt.(scs) →
-      sim_local (r_f) (r ⋅ r')
+      cfg_tgt'.(cst).(scs) = σ_tgt.(scs) → *)
+      sim_fn_body r_f (rc ⋅ r')
                 (fill K_src (of_val v_src)) cfg_src'.(cst)
                 (fill K_tgt (of_val v_tgt)) cfg_tgt'.(cst))
-    : _sim_local sim_local r_f r e_src σ_src
+    : _sim_fn_body sim_fn_body r_f r e_src σ_src
         (fill K_tgt (Call #(LitFnPtr name) el_tgt)) σ_tgt
 (* If tgt prepares to end, src also prepares to end *)
-| sim_local_end_call v_src σ_src v_tgt σ_tgt
+| sim_fn_body_end_call v_src σ_src v_tgt σ_tgt
     (GUAR: ∀ cfg_tgt',
-        ✓ (r ⋅ r_f) →
-        (* wsat (r ⋅ r_f) σ_src σ_tgt → *)
-        φ r c_src cids_entry_src σ_src c_tgt cids_entry_tgt σ_tgt →
+        (* ✓ (r ⋅ r_f) → *)
         (* if tgt can end call *)
         (EndCall (of_val v_tgt), (mkConfig fns_tgt σ_tgt)) ~t~> cfg_tgt' →
         (* then src can also end call *)
-        ∃ cfg_src' r', (EndCall (of_val v_src), (mkConfig fns_src σ_tgt)) ~t~> cfg_src' ∧
+        ∃ cfg_src' r',
+        (EndCall (of_val v_src), (mkConfig fns_src σ_tgt)) ~t~> cfg_src' ∧
         (* and re-establish wsat *)
-        ✓ (r' ⋅ r_f) ∧ wsat (r' ⋅ r_f) cfg_src'.2.(cst) cfg_tgt'.2.(cst) ∧
+        ✓ (r_f ⋅ r') ∧ wsat (r_f ⋅ r') cfg_src'.2.(cst) cfg_tgt'.2.(cst) ∧
         (* and the returned values are related *)
-        vrel (r' ⋅ r_f) (of_val v_src) (of_val v_tgt) ∧
-        (* and call id stacks are restored *)
+        vrel (r_f ⋅ r') (of_val v_src) (of_val v_tgt)
+        (* (* and call id stacks are restored *)
         cfg_src'.2.(cst).(scs) = cids_entry_src ∧
-        cfg_tgt'.2.(cst).(scs) = cids_entry_tgt)
-    : _sim_local sim_local r_f r (EndCall (of_val v_src)) σ_src (EndCall (of_val v_tgt)) σ_tgt
+        cfg_tgt'.2.(cst).(scs) = cids_entry_tgt  *))
+    : _sim_fn_body sim_fn_body r_f r (EndCall (of_val v_src)) σ_src (EndCall (of_val v_tgt)) σ_tgt
 .
 
-Lemma sim_local_mono : monotone6 _sim_local.
+Lemma sim_fn_body_mono : monotone6 _sim_fn_body.
 Proof.
-  intros gσ_f gσ es σs et σt r r' SIM LE; inversion SIM; subst.
-  - by eapply sim_local_stuck; eauto.
-  - eapply sim_local_step. intros et' cfgt' VAL IL STEPT.
-    destruct (STEP _ _ VAL IL STEPT) as (es' & cfgs' & gσ' & STEPS & VAL' & IL' & Hr).
+  intros r_f r es σs et σt R R' SIM LE; inversion SIM; subst.
+  - by eapply sim_fn_body_stuck; eauto.
+  - eapply sim_fn_body_step. intros et' cfgt' STEPT.
+    destruct (STEP _ _ STEPT) as (es' & cfgs' & STEPS & Hr).
     naive_solver.
-  - by eapply sim_local_step_over_call; eauto.
-  - by eapply sim_local_end_call; eauto.
+  - by eapply sim_fn_body_step_over_call; eauto.
+  - by eapply sim_fn_body_end_call; eauto.
 Qed.
 
-Definition sim_local := paco6 _sim_local bot6.
+Definition sim_fn_body := paco6 _sim_fn_body bot6.
 
 End local_step.
 
+Definition sim_fn_body_expr (r: A) (e_src e_tgt: expr) : Prop :=
+  ∀ (r_f: A) (σ_src σ_tgt: state)
+    (VAL: ✓ (r_f ⋅ r)) (INV: wsat (r_f ⋅ r) σ_src σ_tgt),
+  sim_fn_body r_f r e_src σ_src e_tgt σ_tgt.
+
 (* Simulating functions: assuming the calls have been initialized. *)
-Definition sim_local_fn
-  (φ: _ → _ → _ → _ → _ → _ → _ → Prop) (fn_src fn_tgt : function) : Prop :=
-  ∀ (gσ_f gσ : A)
-    (c_src: call_id) (cids_entry_src: call_id_stack)
-    (c_tgt: call_id) (cids_entry_tgt: call_id_stack)
-    el_src el_tgt σ_src σ_tgt e_src e_tgt
+Definition sim_fn_body_fn (r: A) (fn_src fn_tgt : function) : Prop :=
+  ∀ e_src e_tgt el_src el_tgt
     (VALS: Forall (λ ei, terminal ei) el_src)
     (VALT: Forall (λ ei, terminal ei) el_tgt)
-    (VALEQ: Forall2 sim_expr_terminal el_src el_tgt)
+    (VALEQ: Forall2 (vrel r) el_src el_tgt)
     (EQS: match fn_src with
           | FunV xl e => subst_l xl el_src e = Some e_src
           end)
     (EQT: match fn_tgt with
           | FunV xl e => subst_l xl el_tgt e = Some e_tgt
-          end)
-    (VALID: ✓ (gσ ⋅ gσ_f))
-    (INVG: wsat (gσ ⋅ gσ_f) σ_src σ_tgt)
-    (INVL: φ gσ c_src cids_entry_src σ_src c_tgt cids_entry_tgt σ_tgt),
-    sim_local φ c_src cids_entry_src c_tgt cids_entry_tgt
-              gσ_f gσ e_src σ_src e_tgt σ_tgt.
+          end),
+    sim_fn_body_expr r e_src e_tgt.
 
-Definition sim_local_fns : Prop :=
-  ∀ name fn_src, fns_src !! name = Some fn_src → ∃ φ fn_tgt,
-    fns_tgt !! name = Some fn_tgt ∧ sim_local_fn φ fn_src fn_tgt.
+Definition sim_fn_body_fns : Prop :=
+  ∀ name fn_src, fns_src !! name = Some fn_src → ∃ r fn_tgt,
+    fns_tgt !! name = Some fn_tgt ∧ sim_fn_body_fn r fn_src fn_tgt.
+
+Lemma sim_fn_body_resource_mono r_f r1 r2 :
+  r1 ≼ r2 → sim_fn_body r_f r1 <4= sim_fn_body r_f r2.
+Proof.
+  revert r1 r2. pcofix CIH. intros r1 r2 LE es σs et σt SIM.
+  pfold. punfold SIM; [|apply sim_fn_body_mono].
+  inversion SIM; subst.
+  - by eapply sim_fn_body_stuck.
+  - eapply sim_fn_body_step.
+    intros et' ct' STEP'.
+    destruct (STEP _ _ STEP') as (es' & cs' & STEPS' & SIM').
+    exists es', cs'. split; [done|].
+    right. eapply CIH; eauto. by inversion SIM'.
+  - eapply sim_fn_body_step_over_call; eauto.
+    intros vs vt r' cs' ct' VAL WSAT VREL.
+    specialize (RET _ _ _ _ _ VAL WSAT VREL).
+    right. eapply CIH; [eauto|by inversion RET].
+  - eapply sim_fn_body_end_call.
+    intros ct' STEP'. destruct (GUAR _ STEP') as (es' & r' & STEPS' & VAL & WSAT & VREL).
+    naive_solver.
+Qed.
+
 End local.
 
-Hint Resolve sim_local_mono : paco.
+Hint Resolve sim_fn_body_mono : paco.
 
 Section invariant.
   Context {A: cmraT}.
